proof/invariant-abstract/ARM/ArchCSpace_AI.thy
@@ -40,6 +40,30 @@ lemma getActiveIRQ_wp [CSpace_AI_assms]:
   apply (clarsimp simp: irq_state_independent_A_def in_monad return_def split: if_splits)
   done
 
+lemma getCurrentTime_wp[CSpace_AI_assms]:
+  "time_state_independent_A P \<Longrightarrow> getCurrentTime_independent_A P \<Longrightarrow>
+   valid P (do_machine_op getCurrentTime) (\<lambda>_. P)"
+  apply (simp add: getCurrentTime_def do_machine_op_def split_def
+                   select_f_select[simplified liftM_def]
+                   select_modify_comm gets_machine_state_modify)
+  apply wp
+  apply (fastforce simp:time_state_independent_A_def getCurrentTime_independent_A_def in_monad
+                  split: if_splits)
+  done
+
+lemma update_time_stamp_wp[CSpace_AI_assms]:
+  "update_time_stamp_independent_A P \<Longrightarrow> cur_time_independent_A P \<Longrightarrow>
+   time_state_independent_A P \<Longrightarrow> getCurrentTime_independent_A P \<Longrightarrow>
+      valid P update_time_stamp (\<lambda>_. P)"
+  apply (simp add: update_time_stamp_def do_machine_op_def split_def
+                   getCurrentTime_def select_modify_comm gets_machine_state_modify
+                   select_f_select[simplified liftM_def])
+  apply wp
+  apply (fastforce simp: update_time_stamp_independent_A_def cur_time_independent_A_def
+                        time_state_independent_A_def getCurrentTime_independent_A_def in_monad
+                  split: if_splits)
+  done
+
 lemma weak_derived_valid_cap [CSpace_AI_assms]:
   "\<lbrakk> s \<turnstile> c; wellformed_cap c'; weak_derived c' c\<rbrakk> \<Longrightarrow> s \<turnstile> c'"
   apply (case_tac "c = c'", simp)
