proof/invariant-abstract/ARM/ArchRetype_AI.thy
@@ -1309,6 +1309,39 @@ lemma invs_irq_state_independent:
       cur_tcb_def cur_sc_tcb_def sym_refs_def state_refs_of_def
       swp_def valid_irq_states_def valid_replies_pred_pspaceI)
 
+lemma invs_getCurrentTime_independent:
+  "invs (s\<lparr>machine_state := machine_state s\<lparr>time_state := f (time_state (machine_state s))\<rparr>\<rparr>)
+   = invs s"
+  "invs (s\<lparr>machine_state := machine_state s\<lparr>last_machine_time :=
+                            g (last_machine_time (machine_state s)) (time_state (machine_state s))\<rparr>\<rparr>)
+   = invs s"
+  by (clarsimp simp: getCurrentTime_independent_A_def invs_def
+      valid_state_def valid_pspace_def valid_mdb_def valid_ioc_def valid_idle_def
+      only_idle_def if_unsafe_then_cap_def valid_irq_states_def
+      valid_global_refs_def valid_arch_state_def
+      valid_irq_node_def valid_irq_handlers_def valid_machine_state_def
+      valid_arch_caps_def valid_global_objs_def
+      valid_kernel_mappings_def equal_kernel_mappings_def
+      valid_asid_map_def vspace_at_asid_def
+      pspace_in_kernel_window_def cap_refs_in_kernel_window_def
+      cur_tcb_def cur_sc_tcb_def sym_refs_def state_refs_of_def
+      swp_def valid_replies_pred_pspaceI; safe; clarsimp)+
+
+lemma invs_update_time_stamp_independent:
+  "invs (s\<lparr>cur_time := f (cur_time s)\<rparr>) = invs s"
+  "invs (s\<lparr>consumed_time := g (consumed_time s) (cur_time s)\<rparr>) = invs s"
+  by (clarsimp simp: update_time_stamp_independent_A_def invs_def
+      valid_state_def valid_pspace_def valid_mdb_def valid_ioc_def valid_idle_def
+      only_idle_def if_unsafe_then_cap_def valid_irq_states_def
+      valid_global_refs_def valid_arch_state_def
+      valid_irq_node_def valid_irq_handlers_def valid_machine_state_def
+      valid_arch_caps_def valid_global_objs_def
+      valid_kernel_mappings_def equal_kernel_mappings_def
+      valid_asid_map_def vspace_at_asid_def
+      pspace_in_kernel_window_def cap_refs_in_kernel_window_def
+      cur_tcb_def cur_sc_tcb_def sym_refs_def state_refs_of_def
+      swp_def valid_replies_pred_pspaceI; safe; clarsimp)+
+
 crunch irq_masks_inv[wp]: cleanByVA_PoU, storeWord, clearMemory "\<lambda>s. P (irq_masks s)"
   (wp: crunch_wps ignore_del: cleanByVA_PoU storeWord clearMemory)
 
