proof/invariant-abstract/DetSchedDomainTime_AI.thy
@@ -325,8 +325,6 @@ crunch domain_list_inv[wp]: send_signal "\<lambda>s::det_state. P (domain_list s
 
 crunch domain_list_inv[wp]: lookup_reply,lookup_cap "\<lambda>s::det_state. P (domain_list s)"
 
-crunch domain_list_inv[wp]: update_time_stamp "\<lambda>s. P (domain_list s)"
-
 context DetSchedDomainTime_AI_2 begin
 
 lemma invoke_cnode_domain_list_inv[wp]:
@@ -614,8 +612,6 @@ crunch domain_time_inv[wp]: cancel_badged_sends "\<lambda>s::det_state. P (domai
   (ignore: filterM clearMemory
      simp: filterM_mapM crunch_simps
        wp: crunch_wps)
-
-crunch domain_time_inv[wp]: update_time_stamp "\<lambda>s. P (domain_time s)"
 
 context DetSchedDomainTime_AI_2 begin
 
