proof/invariant-abstract/Deterministic_AI.thy
@@ -3972,8 +3972,15 @@ global_interpretation update_work_units_ext_extended: is_extended "update_work_u
 global_interpretation reset_work_units_ext_extended: is_extended "reset_work_units"
   by (unfold_locales; wp)
 
+(*
+time_state_independent_A P; getCurrentTime_independent_A P;
+          update_time_stamp_independent_A P; cur_time_independent_A P;
+*)
+
 lemma preemption_point_inv':
-  "\<lbrakk>irq_state_independent_A P; \<And>f s. P (work_units_completed_update f s) = P s\<rbrakk>
+  "\<lbrakk>irq_state_independent_A P; time_state_independent_A P; getCurrentTime_independent_A P;
+    update_time_stamp_independent_A P; cur_time_independent_A P;
+    \<And>f s. P (work_units_completed_update f s) = P s\<rbrakk>
    \<Longrightarrow> \<lbrace>P\<rbrace> preemption_point \<lbrace>\<lambda>_. P\<rbrace>"
   apply (clarsimp simp: preemption_point_def)
   apply (rule validE_valid)
@@ -3983,7 +3990,7 @@ lemma preemption_point_inv':
   apply (rule alternative_valid; (solves wpsimp)?)
   apply (rule validE_valid)
   apply (rule hoare_seq_ext_skipE, (solves \<open>wpsimp simp: reset_work_units_def\<close>)?)+
-  apply wpsimp
+  apply (wpsimp wp: hoare_vcg_all_lift hoare_drop_imps update_time_stamp_wp)
   done
 
 locale Deterministic_AI_1 =
